pulse/lib/steel/pulse/Pulse.Checker.Bind.fst
@@ -15,33 +15,33 @@ module LN = Pulse.Typing.LN
 module Metatheory = Pulse.Typing.Metatheory
 
 #push-options "--query_stats --ifuel 2 --z3rlimit_factor 4"
-let  mk_bind' (g:env)
-                (pre:term)
-                (e1:st_term)
-                (e2:st_term)
-                (c1:comp_st)
-                (c2:comp_st)
-                (px:nvar { ~ (Set.mem (snd px) (dom g)) })
-                (d_e1:st_typing g e1 c1)
-                (d_c1res:tot_typing g (comp_res c1) (tm_type (comp_u c1)))
-                (d_e2:st_typing (push_binding g (snd px) (fst px) (comp_res c1)) (open_st_term_nv e2 px) c2)
-                (post_hint:post_hint_opt g { comp_post_matches_hint c2 post_hint })
-                (_:squash (
-                    let _, x = px in
-                    comp_pre c1 == pre /\
-                    None? (lookup g x) /\
-                    (~(x `Set.mem` freevars_st e2)) /\
-                    open_term (comp_post c1) x == comp_pre c2))
-  : T.Tac (checker_result_t g pre post_hint)
-   =  let _,x  = px in
-      let s2 = st_comp_of_comp c2 in
-      if x `Set.mem` freevars s2.post
-      then fail g None (Printf.sprintf "Bound variable %d escapes scope in postcondition %s" x (P.term_to_string s2.post))
-      else ( 
-        let res_typing, post_typing = bind_res_and_post_typing g s2 x post_hint  in
-        let (| t, c, d |) = mk_bind g pre e1 e2 c1 c2 px d_e1 d_c1res d_e2 res_typing post_typing in
-        (| t, c, d |)
-      )
+let  mk_bind'
+  (g:env)
+  (pre:term)
+  (e1:st_term)
+  (e2:st_term)
+  (c1:comp_st)
+  (c2:comp_st)
+  (px:nvar { ~ (Set.mem (snd px) (dom g)) })
+  (d_e1:st_typing g e1 c1)
+  (d_c1res:tot_typing g (comp_res c1) (tm_type (comp_u c1)))
+  (d_e2:st_typing (push_binding g (snd px) (fst px) (comp_res c1)) (open_st_term_nv e2 px) c2)
+  (post_hint:post_hint_opt g { comp_post_matches_hint c2 post_hint })
+  (_:squash (let _, x = px in
+             comp_pre c1 == pre /\
+             None? (lookup g x) /\
+             (~(x `Set.mem` freevars_st e2)) /\
+             open_term (comp_post c1) x == comp_pre c2))
+  : T.Tac (checker_result_t g pre post_hint true)
+   = let _,x  = px in
+     let s2 = st_comp_of_comp c2 in
+     if x `Set.mem` freevars s2.post
+     then fail g None (Printf.sprintf "Bound variable %d escapes scope in postcondition %s" x (P.term_to_string s2.post))
+     else ( 
+       let res_typing, post_typing = bind_res_and_post_typing g s2 x post_hint  in
+       let (| t, c, d |) = mk_bind g pre e1 e2 c1 c2 px d_e1 d_c1res d_e2 res_typing post_typing in
+       (| t, c, d |)
+     )
 
 #push-options "--z3rlimit_factor 4 --fuel 0 --ifuel 1"
 let check_bind
@@ -50,10 +50,13 @@ let check_bind
   (pre:term)
   (pre_typing:tot_typing g pre tm_vprop)
   (post_hint:post_hint_opt g)
+  (frame_pre:bool)
   (check:check_t)
-  : T.Tac (checker_result_t g pre post_hint) =
+  : T.Tac (checker_result_t g pre post_hint frame_pre) =
+  if not frame_pre
+  then T.fail "check_bind: frame_pre is false, bailing";
   let Tm_Bind { binder=b; head=e1; body=e2 } = t.term in
-  let (| e1, c1, d1 |) = check g e1 pre pre_typing None in
+  let (| e1, c1, d1 |) = check g e1 pre pre_typing None frame_pre in
   if not (stateful_comp c1)
   then fail g None "Bind: c1 is not st"
   else 
@@ -64,7 +67,7 @@ let check_bind
     let px = b.binder_ppname, x in
     let next_pre = open_term_nv s1.post px in
     let g' = push_binding g x b.binder_ppname s1.res in
-    let (| e2', c2, d2 |) = check g' (open_st_term_nv e2 px) next_pre next_pre_typing post_hint in
+    let (| e2', c2, d2 |) = check g' (open_st_term_nv e2 px) next_pre next_pre_typing post_hint frame_pre in
     FV.st_typing_freevars d2;
     if not (stateful_comp c2)
     then fail g None "Bind: c2 is not st"
@@ -76,8 +79,9 @@ let check_bind
 //inlining mk_bind' causes memory to blow up. F* takes a long time to compute a VC for the definition above^. Z3 finishes the proof quickly    
 #pop-options
 
-
-let check_tot_bind g t pre pre_typing post_hint check =
+let check_tot_bind g t pre pre_typing post_hint frame_pre check =
+  if not frame_pre
+  then T.fail "check_tot_bind: frame_pre is false, bailing";
   let Tm_TotBind { head=e1; body=e2 } = t.term in
   let (| e1, u1, t1, _t1_typing, e1_typing |) = check_term_and_type g e1 in
   let t1 =
@@ -95,7 +99,7 @@ let check_tot_bind g t pre pre_typing post_hint check =
   let pre_typing' : tot_typing g' pre tm_vprop =
     check_vprop_with_core g' pre in
   let (| e2, c2, e2_typing |) =
-    check g' (open_st_term_nv e2 px) pre pre_typing' post_hint in
+    check g' (open_st_term_nv e2 px) pre pre_typing' post_hint frame_pre in
   if not (stateful_comp c2)
   then fail g (Some e2.range) "Tm_TotBind: e2 is not a stateful computation"
   else
@@ -123,11 +127,11 @@ let check_tot_bind g t pre pre_typing post_hint check =
 
 let coerce_eq (#a #b:Type) (x:a) (_:squash (a == b)) : y:b{y == x} = x
 
-let check_stapp_no_ctxt (g:env) (t:st_term { Tm_STApp? t.term })
-  : T.Tac (uvs : env { disjoint uvs g } &
-           t:st_term &
-           c:comp_st &
-           st_typing (push_env g uvs) t c) = magic ()
+// let check_stapp_no_ctxt (g:env) (t:st_term { Tm_STApp? t.term })
+//   : T.Tac (uvs : env { disjoint uvs g } &
+//            t:st_term &
+//            c:comp_st &
+//            st_typing (push_env g uvs) t c) = magic ()
 
 module PS = Pulse.Prover.Substs
 open Pulse.Prover.Common
@@ -139,16 +143,25 @@ let check_bindv2
   (pre:term)
   (pre_typing:tot_typing g pre tm_vprop)
   (post_hint:post_hint_opt g)
+  (frame_pre:bool)
   (check:check_t)
-  : T.Tac (checker_result_t g pre post_hint) =
+  : T.Tac (checker_result_t g pre post_hint frame_pre) =
+
+  if not frame_pre
+  then T.fail "check_bindv2: frame_pre is not set, bailing";
 
   let Tm_Bind { binder=b; head=e1; body=e2 } = t.term in
 
   match e1.term with
   | Tm_STApp _ ->
-    let (| uvs, e1, c1, d1 |) = check_stapp_no_ctxt g e1 in
+    // let (| uvs, e1, c1, d1 |) =
+    let (| e1, c1, d1 |) =
+      check g e1 pre pre_typing None false in
+    let uvs = mk_env (fstar_env g) in
+      // check_stapp_no_ctxt g e1 in
     let c10 = c1 in
-    // magic is comp_pre c1 typing, get from inversion of d1 
+    // magic is comp_pre c1 typing, get from inversion of d1
+    assume (stateful_comp c1);
     let (| g1, uvs1, ss1, remaining_pre, k |) =
       prove pre_typing uvs #(comp_pre c1) (magic ()) in
     let x = fresh g1 in
@@ -162,11 +175,12 @@ let check_bindv2
     // remaining_pre is well-typed, may be prove function can return it?
     // well-typedness of open_term?
     let (| e2, c2, d2 |) =
-      check g2 (open_st_term_nv e2 px) pre_e2 (magic ()) (extend_post_hint_opt_g g post_hint g2) in
+      check g2 (open_st_term_nv e2 px) pre_e2 (magic ()) (extend_post_hint_opt_g g post_hint g2) frame_pre in
     
     if not (stateful_comp c2)
     then fail g None "Bind: c2 is not st"
     else
+      let _ = assert (equal g (push_env g uvs)) in
       let d1 = st_typing_weakening g uvs e1 c1 d1 g1 in
       let d1 = st_typing_weakening_end g1 uvs e1 c1 d1 uvs1 in
       let d1 = PS.st_typing_nt_substs_derived g1 uvs1 #e1 #c1 d1 ss1 in
