pulse/lib/steel/pulse/Pulse.Checker.Bind.fsti
@@ -9,13 +9,15 @@ open Pulse.Elaborate.Pure
 open Pulse.Typing
 open Pulse.Checker.Common
 
-val check_bind (g:env)
-               (t:st_term{Tm_Bind? t.term})
-               (pre:term)
-               (pre_typing:tot_typing g pre tm_vprop)
-               (post_hint:post_hint_opt g)               
-               (check:check_t)
-  : T.Tac (checker_result_t g pre post_hint)
+val check_bind
+  (g:env)
+  (t:st_term{Tm_Bind? t.term})
+  (pre:term)
+  (pre_typing:tot_typing g pre tm_vprop)
+  (post_hint:post_hint_opt g)
+  (frame_pre:bool)
+  (check:check_t)
+  : T.Tac (checker_result_t g pre post_hint frame_pre)
 
 val check_tot_bind
   (g:env)
@@ -23,5 +25,7 @@ val check_tot_bind
   (pre:term)
   (pre_typing:tot_typing g pre tm_vprop)
   (post_hint:post_hint_opt g)
+  (frame_pre:bool)
   (check:check_t)
-  : T.Tac (checker_result_t g pre post_hint)
+  : T.Tac (checker_result_t g pre post_hint frame_pre)
+
