pulse/lib/steel/pulse/Pulse.Checker.Exists.fsti
@@ -12,7 +12,8 @@ val check_elim_exists
   (pre:term)
   (pre_typing:tot_typing g pre tm_vprop)
   (post_hint:post_hint_opt g)
-  : T.Tac (checker_result_t g pre post_hint)
+  (frame_pre:bool)
+  : T.Tac (checker_result_t g pre post_hint frame_pre)
 
 let intro_exists_witness_singleton (st:st_term)  = 
   match st.term with
@@ -30,4 +31,5 @@ val check_intro_exists_either
   (pre:term)
   (pre_typing:tot_typing g pre tm_vprop)
   (post_hint:post_hint_opt g)
-  : T.Tac (checker_result_t g pre post_hint)
+  (frame_pre:bool)
+  : T.Tac (checker_result_t g pre post_hint frame_pre)
